\documentclass[11pt,letterpaper]{article}
\usepackage[lmargin=1in,rmargin=1in,tmargin=1in,bmargin=1in]{geometry}
\usepackage{../style/homework}
\setbool{quotetype}{true} % True: Side; False: Under
\setbool{hideans}{false} % Student: True; Instructor: False

\usepackage{cancel} % Use Cancel

% -------------------
% Content
% -------------------
\begin{document}

\homework{3: Due 01/31}{And I knew exactly what to do\dots but in a much more real sense, I had no idea what to do.}{Michael Scott, The Office}

% Problem 1
\problem{10} Showing all your work, simplify the following as much as possible (express any denominators using negative powers):
	\begin{enumerate}[(a)]
	\item $\dfrac{x^5 y^3}{x^3 y^9}$
	\item $\dfrac{(x^2 y^{-3})^4}{x^0 y^2}$
	\item $\dfrac{(x^8 y^3)^0 x y^7}{(x^2)^3 y}$
	\end{enumerate} \pspace

\sol 
\begin{enumerate}[(a)]
\item 
	\[
	\dfrac{x^5 y^3}{x^3 y^9}= \dfrac{x^{\cancel{5}^{\,2}} \cancel{y^3}}{\cancel{x^3} y^{\cancel{9}^{\,6}}}= \dfrac{x^2}{y^6}= x^2 y^{-6}
	\] \pspace

\item 
	\[
	\dfrac{(x^2 y^{-3})^4}{x^0 y^2}= \dfrac{x^8 y^{-12}}{1 \cdot y^2}= \dfrac{x^8}{y^{12} y^2}= \dfrac{x^8}{y^{14}}= x^8 y^{-14}
	\] \pspace

\item 
	\[
	\dfrac{(x^8 y^3)^0 x y^7}{(x^2)^3 y}= \dfrac{1 \cdot x y^7}{x^6 y}= \dfrac{\cancel{x} y^{\cancel{7}^{\,6}}}{x^{\cancel{6}^{\,5}} \cancel{y}}= \dfrac{y^6}{x^5}= y^6 x^{-5}
	\]
\end{enumerate}



\newpage



% Problem 2
\problem{10} Showing all your work, simplify the following as much as possible (do not express your answer using any negative powers): 
	\begin{enumerate}[(a)]
	\item $\dfrac{x^{-2} y z^6}{x y^{-6} z^5}$
	\item $\dfrac{(x y^{-2})^{-1}}{x^3 y^{-7}}$
	\item $\left( \dfrac{x^5 y^{-4}}{(x^{-4} y^3)^{-8}} \right)^0$
	\end{enumerate} \pspace

\sol 
\begin{enumerate}[(a)]
\item 
	\[
	\dfrac{x^{-2} y z^6}{x y^{-6} z^5}= \dfrac{y^6 y z^6}{x^2 x z^5}= \dfrac{y^7 z^6}{x^3 z^5}= \dfrac{y^7 z^{\cancel{6}^{\,1}}}{x^3 \cancel{z^5}}= \dfrac{y^7 z}{x^3}
	\] \pspace

\item 
	\[
	\dfrac{(x y^{-2})^{-1}}{x^3 y^{-7}}= \dfrac{x^{-1} y^2}{x^3 y^{-7}}= \dfrac{y^7 y^2}{x^1 x^3}= \dfrac{y^9}{x^4}
	\] \pspace

\item 
	\[
	\left( \dfrac{x^5 y^{-4}}{(x^{-4} y^3)^{-8}} \right)^0= 1
	\]
\end{enumerate}



\newpage



% Problem 3
\problem{10} Showing all your work, simplify the following as much as possible (do not express your answer using any negative powers): 
	\[
	\dfrac{\left( (x y z)^5 x z^{-4} \right)^2 x^{-5}}{x y^{-3} z^{-2}}
	\] \pspace

\sol 
	\[
	\begin{gathered}
	\dfrac{\left( (x y z)^5 x z^{-4} \right)^2 x^{-5}}{x y^{-3} z^{-2}} \\[0.3cm]
	\dfrac{\big( x^5 y^5 z^5 x z^{-4} \big)^2 x^{-5}}{x y^{-3} z^{-2}} \\[0.3cm]
	\dfrac{ \big(x^6 y^5 z^1 \big)^2 x^{-5}}{x y^{-3} z^{-2}} \\[0.3cm]
	\dfrac{x^{12} y^{10} z^2 x^{-5}}{x y^{-3} z^{-2}} \\[0.3cm]
	\dfrac{x^7 y^{10} z^2 y^3 z^2}{x} \\[0.3cm] 
	\dfrac{x^7 y^{13} z^4}{x} \\[0.3cm]
	\dfrac{x^{\cancel{7}^{\,6}} y^{13} z^4}{\cancel{x}} \\[0.3cm]
	x^6 y^{13} z^4
	\end{gathered}
	\]


\end{document}