\documentclass[11pt,letterpaper]{article}
\usepackage[lmargin=1in,rmargin=1in,tmargin=1in,bmargin=1in]{geometry}
\usepackage{../style/homework}
\usepackage{../style/commands}
\setbool{quotetype}{true} % True: Side; False: Under
\setbool{hideans}{false} % Student: True; Instructor: False

% -------------------
% Content
% -------------------
\begin{document}

\homework{16: Due 12/06}{Algebra is the metaphysics of arithmetic.}{John Ray}

% Problem 1
\problem{10} Let $\mathbf{u}, \mathbf{v} \in \mathbb{R}^4$ be defined by $\mathbf{u}= \begin{pmatrix} 1 \\ 0 \\ -3 \\ 2 \end{pmatrix}$ and $\mathbf{v}= \begin{pmatrix} 4 \\ -1 \\ 6 \\ -5 \end{pmatrix}$. Showing all your work, compute the following:
	\begin{enumerate}[(a)]
	\item $-6 \mathbf{u}$
	\item $\mathbf{v} - \mathbf{u}$
	\item $\mathbf{u} + 2 \mathbf{v}$
	\item $\mathbf{u} \cdot \mathbf{v}$
	\end{enumerate} \pspace

\sol 
\begin{enumerate}[(a)]
\item 
	\[
	-6 \mathbf{u}= -6 \begin{pmatrix} 1 \\ 0 \\ -3 \\ 2 \end{pmatrix}= \begin{pmatrix} -6 \\ 0 \\ 18 \\ -12 \end{pmatrix}
	\]

\item 
	\[
	\mathbf{v} - \mathbf{u}= \begin{pmatrix} 4 \\ -1 \\ 6 \\ -5 \end{pmatrix} - \begin{pmatrix} 1 \\ 0 \\ -3 \\ 2 \end{pmatrix}= \begin{pmatrix} 3 \\ -1 \\ 9 \\ -7 \end{pmatrix}
	\]

\item 
	\[
	\mathbf{u} + 2 \mathbf{v}=  \begin{pmatrix} 1 \\ 0 \\ -3 \\ 2 \end{pmatrix} + 2 \begin{pmatrix} 4 \\ -1 \\ 6 \\ -5 \end{pmatrix}=  \begin{pmatrix} 1 \\ 0 \\ -3 \\ 2 \end{pmatrix} + \begin{pmatrix} 8 \\ -2 \\ 12 \\ -10 \end{pmatrix}= \begin{pmatrix} 9 \\ -2 \\ 9 \\ -8 \end{pmatrix}
	\]

\item 
	\[
	\mathbf{u} \cdot \mathbf{v}= \begin{pmatrix} 1 \\ 0 \\ -3 \\ 2 \end{pmatrix} \cdot \begin{pmatrix} 4 \\ -1 \\ 6 \\ -5 \end{pmatrix}= 1(4) + 0(-1) + (-3)6 + 2(-5)= 4 + 0 - 18 - 10= -24
	\]
\end{enumerate}



\newpage



% Problem 2
\problem{10} Define matrices $A, B, C$ as follows:
	\[
	A= \begin{pmatrix} 1 & 0 & -4 \\ -2 & 3 & 1 \end{pmatrix}, \qquad B= \begin{pmatrix} 0 & 2 & -2 \\ 5 & 1 & 4 \end{pmatrix}, \qquad C= \begin{pmatrix} 2 & 0 \\ -1 & 6 \\ 5 & 3 \end{pmatrix}
	\]
Showing all your work, compute the following:
	\begin{enumerate}[(a)]
	\item $4A$
	\item $A - B$
	\item $3A + B$
	\item $AC$
	\item $B^T$
	\end{enumerate} \pspace

\sol 
\begin{enumerate}[(a)]
\item 
	\[
	4 \begin{pmatrix} 1 & 0 & -4 \\ -2 & 3 & 1 \end{pmatrix}= \begin{pmatrix} 4 & 0 & -16 \\ -8 & 12 & 4 \end{pmatrix}
	\]

\item 
	\[
	\begin{pmatrix} 1 & 0 & -4 \\ -2 & 3 & 1 \end{pmatrix} - \begin{pmatrix} 0 & 2 & -2 \\ 5 & 1 & 4 \end{pmatrix}= \begin{pmatrix} 1 & -2 & -2 \\ -7 & 2 & -3 \end{pmatrix}
	\]

\item 
	\[
	3 \begin{pmatrix} 1 & 0 & -4 \\ -2 & 3 & 1 \end{pmatrix} + \begin{pmatrix} 0 & 2 & -2 \\ 5 & 1 & 4 \end{pmatrix}= \begin{pmatrix} 3 & 0 & -12 \\ -6 & 9 & 3 \end{pmatrix} + \begin{pmatrix} 0 & 2 & -2 \\ 5 & 1 & 4 \end{pmatrix}= \begin{pmatrix} 3 & 2 & -14 \\ -1 & -8 & 7 \end{pmatrix}
	\]

\item 
	\[
	\begin{pmatrix} 1 & 0 & -4 \\ -2 & 3 & 1 \end{pmatrix} \begin{pmatrix} 2 & 0 \\ -1 & 6 \\ 5 & 3 \end{pmatrix}= \begin{pmatrix} 1(2) + 0(-1) + (-4)5 & 1(0) + 0(6) + (-4)3 \\ -2(2) + 3(-1) + 1(5) & -2(0) + 3(6) + 1(3) \end{pmatrix}= \begin{pmatrix} -18 & -12 \\ -2 & 21 \end{pmatrix}
	\]
	
\item 
	\[
	\begin{pmatrix} 0 & 2 & -2 \\ 5 & 1 & 4 \end{pmatrix}^T= \begin{pmatrix} 0 & 5 \\ 2 & 1 \\ -2 & 4 \end{pmatrix}
	\]
\end{enumerate}



\newpage



% Problem 3
\problem{10} Define matrices $A, B, C$ as follows:
	\[
	A= \begin{pmatrix} 1 & 0 & 2 \\ 0 & -1 & 3 \end{pmatrix}, \qquad B= \begin{pmatrix} 2 & -1 \\ 0 & 3 \end{pmatrix}, \qquad C= \begin{pmatrix} 0 & 1 & 0 \\ 1 & 0 & 0 \\ 0 & 0 & 1 \end{pmatrix}
	\]
Showing all your work and explaining your reasoning, answer the following:
        \begin{enumerate}[(a)]
        \item What is $B^2$?
        \item If $CA$ is defined, compute it. If not, explain why. 
        \item What is $a_{23}$? What is $b_{21}$?
        \item If $M= AC$, without explicitly computing $AC$, what is $m_{23}$?
        \end{enumerate} \pspace

\sol 
\begin{enumerate}[(a)]
\item We have\dots
	\[
	\begin{aligned}
	B^2= \begin{pmatrix} 2 & -1 \\ 0 & 3 \end{pmatrix}^2= \begin{pmatrix} 2 & -1 \\ 0 & 3 \end{pmatrix} \begin{pmatrix} 2 & -1 \\ 0 & 3 \end{pmatrix}= \begin{pmatrix} 2(2) + (-1)0 & 2(-1) + (-1)3 \\ 0(2) + 3(0) & 0(-1) + 3(3) \end{pmatrix}= \begin{pmatrix} 4 & -5 \\ 0 & 9 \end{pmatrix}
	\end{aligned}
	\]

\item The product $CA$ is not defined. The product of two matrices, say $AB$, where $A$ is a $m \times n$ matrix and $B$ is a $r \times s$ matrix, is defined if and only if $n= r$. Here, we have $m= n= 3$ and $r= 2$ and $s= 3$. Because $n= 3 \neq 2= r$, the product is not defined. 

\item We have $a_{23}= 3$ and $b_{21}= 1$. 

\item We know $m_{23}$ is the dot product of the second row of $A$ with the third column of $C$. But then we have\dots
	\[
	m_{23}= 0(0) + (-1)0 + 3(3)= 0 + 0 + 9= 9
	\]
\end{enumerate}



\newpage



% Problem 4
\problem{10} If $A, B$ are matrices, is it true $(A + B)^2= A^2 + 2AB + B^2$? If so, explain why. If not, explain why not. \pspace

\sol The statement is false. Matrix multiplication is not commutative. 


\end{document}