\documentclass[11pt,letterpaper]{article}
\usepackage[lmargin=1in,rmargin=1in,tmargin=1in,bmargin=1in]{geometry}
\usepackage{../style/homework}
\usepackage{../style/commands}
\setbool{quotetype}{false} % True: Side; False: Under
\setbool{hideans}{false} % Student: True; Instructor: False

% -------------------
% Content
% -------------------
\begin{document}

\homework{2: Due 01/05}{I don't talk trash, I talk smack. They're totally different. Trash talk is hypothetical, like: your mom is so fat she can eat the internet. But smack talk is happening like right now. Like: you're ugly and I know it for a fact 'cause I got the evidence right there.}{Kelly Kapoor, The Office}

% Problem 1
\problem{10} Showing all your work, simplify the following as much as possible:
\begin{enumerate}[(a)]
\item $(x^3 y^{-1})^4$
\item $\dfrac{x^5y^{-6}}{x^3y^2}$
\item $\left( \dfrac{x^{-2}}{y^4} \right)^{-1}$
\item $\dfrac{(xy)^0 x^{-3}}{(y^2)^3}$
\item $\dfrac{(x^{-2} y^3)^{-5} xy^6}{x^0 y^{-2}}$
\end{enumerate} \pspace

\sol
\begin{enumerate}[(a)]
\item 
	\[
	(x^3 y^{-1})^4= x^12 y^{-4}= \dfrac{x^{12}}{y^4}
	\] \pspace

\item 
	\[
	\dfrac{x^5y^{-6}}{x^3y^2}= \dfrac{x^5}{x^3 y^2 y^6}= \dfrac{x^5}{x^3 y^8}= \dfrac{x^2}{y^8}
	\] \pspace

\item 
	\[
	\left( \dfrac{x^{-2}}{y^4} \right)^{-1}= \dfrac{y^4}{x^{-2}}= x^2 y^4
	\] \pspace

\item 
	\[
	\dfrac{(xy)^0 x^{-3}}{(y^2)^3}= \dfrac{1 \cdot x^{-3}}{y^6}= \dfrac{1}{x^3 y^6}
	\] \pspace

\item 
	\[
	\dfrac{(x^{-2} y^3)^{-5} xy^6}{x^0 y^{-2}}= \dfrac{x^{10} y^{-15} x y^6}{1 \cdot y^{-2}}= \dfrac{x^{10} x y^6 y^2}{y^{15}}= \dfrac{x^{11} y^8}{y^{15}}= \dfrac{x^{11}}{y^7}
	\]
\end{enumerate}



\newpage



% Problem 2
\problem{10} Showing all your work, simplify the following as much as possible:
\begin{enumerate}[(a)]
\item $(x^4 y^5)^{1/2}$
\item $\left( \dfrac{\sqrt{x}}{\sqrt[3]{y^2}} \right)^3$
\item $\dfrac{(x \sqrt{y})^{3}}{\sqrt{x}\, y^{-3/2}}$
\item $(\sqrt[3]{x y^2})^2 (xy^2)^{1/3}$
\item $\left( \dfrac{x^6}{y^5} \right)^{-2/3}$
\end{enumerate} \pspace

\sol
\begin{enumerate}[(a)]
\item 
	\[
	(x^4 y^5)^{1/2}= x^{4/2} y^{5/2}= x^2 y^{5/2}= x^2 \sqrt{y^5}
	\] \pspace

\item 
	\[
	\left( \dfrac{\sqrt{x}}{\sqrt[3]{y^2}} \right)^3= \left( \dfrac{x^{1/2}}{y^{2/3}} \right)^3= \dfrac{x^{3/2}}{y^2}= \dfrac{\sqrt[3]{x^2}}{y^2}
	\] \pspace

\item 
	\[
	\dfrac{(x \sqrt{y})^{3}}{\sqrt{x}\, y^{-3/2}}= \dfrac{(x y^{1/2})^{3}}{x^{1/2} y^{-3/2}}= \dfrac{x^3 y^{3/2} \cdot y^{3/2}}{x^{1/2}}= \dfrac{x^3 y^3}{x^{1/2}}= x^{5/2} y^3= y^3 \sqrt{x^5}
	\] \pspace

\item 
	\[
	(\sqrt[3]{x y^2})^2 (xy^2)^{1/3}= (x^{1/3} y^{2/3})^2 (xy^2)^{1/3}= x^{2/3} y^{4/3} x^{1/3} y^{2/3}= x^1 y^{6/3}= xy^2
	\] \pspace

\item 
	\[
	\left( \dfrac{x^6}{y^5} \right)^{-2/3}= \left( \dfrac{y^5}{x^6} \right)^{2/3}= \dfrac{y^{10/3}}{x^{12/3}}= \dfrac{y^{10/3}}{x^4}= \dfrac{\sqrt[3]{y^{10}}}{x^4}
	\] 
\end{enumerate}



\newpage



% Problem 3
\problem{10} Showing all your work, simplify the following as much as possible:
\begin{enumerate}[(a)]
\item $\sqrt{28}$
\item $\sqrt{120}$
\item $\dfrac{\sqrt{90}}{3}$
\item $\sqrt[3]{360}$
\item $\sqrt[4]{2^9 \cdot 3^5 \cdot 5^2 \cdot 7^4}$
\end{enumerate} \pspace

\sol
\begin{enumerate}[(a)]
\item 
	\[
	\sqrt{28}= \sqrt{2^2 \cdot 7}= 2 \sqrt{7}
	\] \pspace

\item 
	\[
	\sqrt{120}= \sqrt{2^3 \cdot 3 \cdot 5}= 2 \sqrt{2 \cdot 3 \cdot 5}= 2\sqrt{30}
	\] \pspace

\item 
	\[
	\dfrac{\sqrt{90}}{3}= \dfrac{\sqrt{2 \cdot 3^2 \cdot 5}}{3}= \dfrac{3 \sqrt{2 \cdot 5}}{3}= \sqrt{10}
	\] \pspace

\item 
	\[
	\sqrt[3]{360}= \sqrt[3]{2^3 \cdot 3^2 \cdot 5}= 2 \sqrt[3]{3^2 \cdot 5}= 2 \sqrt[3]{45}
	\] \pspace

\item 
	\[
	\sqrt[4]{2^9 \cdot 3^5 \cdot 5^2 \cdot 7^4}= 2^2 \cdot 3^1 \cdot 7 \sqrt[4]{2 \cdot 3 \cdot 5^2}= 84 \sqrt[4]{150}
	\]
\end{enumerate}



\newpage



% Problem 4
\problem{10} Rationalize the following fractions:
\begin{enumerate}[(a)]
\item $\dfrac{1}{\sqrt{3}}$
\item $\dfrac{6}{\sqrt{5}}$
\item $\dfrac{4}{1 + \sqrt{6}}$
\item $\dfrac{6}{3 - \sqrt{7}}$
\item $\dfrac{1}{\sqrt[3]{12}}$
\end{enumerate} \pspace

\sol
\begin{enumerate}[(a)]
\item 
	\[
	\dfrac{1}{\sqrt{3}}= \dfrac{1}{\sqrt{3}} \cdot \dfrac{\sqrt{3}}{\sqrt{3}}= \dfrac{\sqrt{3}}{3}
	\] \pspace

\item 
	\[
	\dfrac{6}{\sqrt{5}}= \dfrac{6}{\sqrt{5}} \cdot \dfrac{\sqrt{5}}{\sqrt{5}}= \dfrac{6\sqrt{5}}{5}
	\] \pspace

\item 
	\[
	\dfrac{4}{1 + \sqrt{6}}= \dfrac{4}{1 + \sqrt{6}} \cdot \dfrac{1 - \sqrt{6}}{1 - \sqrt{6}}= \dfrac{4 - 4\sqrt{6}}{1 - \sqrt{6} + \sqrt{6} - 6}= \dfrac{4 - 4\sqrt{6}}{-5}= \dfrac{4\sqrt{6} - 4}{5}
	\]

\item 
	\[
	\dfrac{6}{3 - \sqrt{7}}= \dfrac{6}{3 - \sqrt{7}} \cdot \dfrac{3 + \sqrt{7}}{3 + \sqrt{7}}= \dfrac{18 + 6\sqrt{7}}{9 + 3\sqrt{7} - 3\sqrt{7} - 7}= \dfrac{18 + 6\sqrt{7}}{2}= 9 + 3\sqrt{7}
	\] \pspace

\item 
	\[
	\dfrac{1}{\sqrt[3]{12}}= \dfrac{1}{(12)^{1/3}} \cdot \dfrac{(12)^{2/3}}{(12)^{2/3}}= \dfrac{(12^{2/3}}{12}= \dfrac{\sqrt[3]{12^2}}{12}= \dfrac{\sqrt[3]{144}}{12}= \dfrac{\sqrt[3]{8 \cdot 18}}{12}= \dfrac{2\sqrt[3]{18}}{12}= \dfrac{\sqrt[3]{18}}{6}
	\]
\end{enumerate}



\newpage



% Problem 5
\problem{10} Convert the following numbers from scientific to decimal notation:
\begin{enumerate}[(a)]
\item $1.5 \cdot 10^4$
\item $3.19 \cdot 10^{-3}$
\item $-4.33 \cdot 10^0$
\item $1.574 \cdot 10^2$
\item $8.48 \cdot 10^{-6}$
\end{enumerate} \pspace

\sol
\begin{enumerate}[(a)]
\item $1.5 \cdot 10^4= 15000$
\item $3.19 \cdot 10^{-3}= 0.00319$
\item $-4.33 \cdot 10^0= -4.33$
\item $1.574 \cdot 10^2= 157.4$
\item $8.48 \cdot 10^{-6}= 0.00000848$
\end{enumerate}



\newpage



% Problem 6
\problem{10} Convert the following numbers from decimal to scientific notation:
\begin{enumerate}[(a)]
\item $14500000$
\item $0.004$
\item $878410$
\item $0.0000077$
\item $1.55$
\end{enumerate} \pspace

\sol
\begin{enumerate}[(a)]
\item $14500000= 1.45 \cdot 10^7$
\item $0.004= 4.0 \cdot 10^{-3}$
\item $878410= 8.78410 \cdot 10^5$
\item $0.0000077= 7.7 \cdot 10^{-6}$
\item $1.55= 1.55 \cdot 10^0$
\end{enumerate}



\newpage



% Problem 7
\problem{10} Express the following rational numbers as a decimal:
\begin{enumerate}[(a)]
\item $\dfrac{3}{8}$
\item $\dfrac{13}{4}$
\item $\dfrac{4}{5}$
\item $\dfrac{1}{9}$
\item $\dfrac{4}{33}$
\end{enumerate} \pspace

\sol \par
\begin{minipage}{0.48\textwidth}
\begin{enumerate}[(a)]
\item $\dfrac{3}{8}: \longdivision{3}{8}$. Then $\frac{3}{8}= 0.375$.
\item $\dfrac{13}{4}: \longdivision{13}{4}$. Then $\frac{13}{4}= 3.25$.
\item $\dfrac{4}{5}: \longdivision{4}{5}$. Then $\frac{4}{5}= 0.8$.
\end{enumerate}
\end{minipage}%
\begin{minipage}{0.48\textwidth}
\begin{enumerate}
\item[(d)] $\dfrac{1}{9}: \longdivision{1}{9}$. Then $\frac{1}{9}= 0.\overline{1}$.
\item[(e)] $\dfrac{4}{33}: \longdivision{4}{33}$. Then $\frac{4}{33}= 0.\overline{12}$.
\end{enumerate}
\end{minipage}



\newpage



% Problem 8
\problem{10} Express the following decimal numbers as rational numbers:
\begin{enumerate}[(a)]
\item $-6$
\item $1.4$
\item $0.54$
\item $0.2222\overline{2}$
\item $0.1010\overline{10}$
\end{enumerate} \pspace

\sol
\begin{enumerate}[(a)]
\item 
	\[
	-6= \dfrac{-6}{1}
	\] \pspace

\item 
	\[
	1.4= \dfrac{14}{10}= \dfrac{7}{5}
	\] \pspace

\item 
	\[
	0.54= \dfrac{54}{100}= \dfrac{27}{50}
	\] \pspace

\item \phantom{.} \par
	\begin{table}[!ht]
	\centering\small
	\begin{tabular}{ccc}
	$10N$ & $=$ & $2.2222\overline{2}$ \\ 
	$N$ & $=$ & $0.2222\overline{2}$ \\ \hline
	$9N$ & $=$ & $2$ \\
	& $N= \frac{2}{9}$ & 
	\end{tabular}
	\end{table}

\item \phantom{.} \par
	\begin{table}[!ht]
	\centering\small
	\begin{tabular}{ccc}
	$100N$ & $=$ & $10.1010\overline{10}$ \\ 
	$N$ & $=$ & $0.1010\overline{10}$ \\ \hline
	$99N$ & $=$ & $10$ \\
	& $N= \frac{10}{99}$ & 
	\end{tabular}
	\end{table} 
\end{enumerate}



\newpage



% Problem 9
\problem{10} Showing all your work, compute the following:
\begin{enumerate}[(a)]
\item $(1 - 5i) + (6 + 8i)$
\item $(5 + 6i) - 2(4 - i)$
\item $(3 + i)(4 + 2i)$
\item $\dfrac{1 + i}{8 + i}$
\item $(5 - 3i)^2$
\end{enumerate} \pspace

\sol
\begin{enumerate}[(a)]
\item 
	\[
	(1 - 5i) + (6 + 8i)= (1 + 6) + (-5i + 8i)= 7 + 3i
	\] \pspace

\item 
	\[
	(5 + 6i) - 2(4 - i)= (5 + 6i) + (-8 + 2i)= (5 - 8) + (6i + 2i)= -3 + 8i
	\] \pspace

\item 
	\[
	(3 + i)(4 + 2i)= 12 + 6i + 4i + 2i^2= 12 + 10i - 2= 10 + 10i
	\] \pspace

\item 
	\[
	\dfrac{1 + i}{8 + i}= \dfrac{1 + i}{8 + i} \cdot \dfrac{8 - i}{8 - i}= \dfrac{(1 + i)(8 - i)}{(8 + i)(8 - i)}= \dfrac{8 - i + 8i - i^2}{64 - 8i + 8i - i^2}= \dfrac{8 + 7i + 1}{64 + 1}= \dfrac{9 + 7i}{65}= \frac{9}{65} + \frac{7}{65}\,i
	\] \pspace

\item 
	\[
	(5 - 3i)^2= (5 - 3i)(5 - 3i)= 25 - 15i -15i + 9i^2= 25 - 30i - 9= 16 - 30i
	\]
\end{enumerate}



\newpage



% Problem 10
\problem{10} Simplifying as much as possible, express the following as a single complex number of the form $a + bi$:
\begin{enumerate}[(a)]
\item $7$
\item $\sqrt{-4}$
\item $6 - \sqrt{-18}$
\item $(2i)^3$
\item $\dfrac{1 + \sqrt{-9}}{3}$
\end{enumerate} \pspace

\sol
\begin{enumerate}[(a)]
\item 
	\[
	7= 7 + 0i
	\] \pspace

\item 
	\[
	\sqrt{-4}= \sqrt{4} i= 2i= 0 + 2i
	\] \pspace

\item 
	\[
	6 - \sqrt{-18}= 6 - \sqrt{18}i= 6 - \sqrt{9 \cdot 2}i= 6 - 3\sqrt{2}i
	\] \pspace

\item 
	\[
	(2i)^3= 2^3 i^3= 8(-i)= -8i= 0 - 8i
	\] \pspace

\item 
	\[
	\dfrac{1 + \sqrt{-9}}{3}= \dfrac{1 + \sqrt{9}i}{3}= \dfrac{1 + 3i}{3}= \frac{1}{3} + i
	\]
\end{enumerate}


\end{document}