\documentclass[11pt,letterpaper]{article}
\usepackage[lmargin=1in,rmargin=1in,tmargin=1in,bmargin=1in]{geometry}
\usepackage{../style/homework}
\usepackage{../style/commands}
\setbool{quotetype}{false} % True: Side; False: Under
\setbool{hideans}{false} % Student: True; Instructor: False

% -------------------
% Content
% -------------------
\begin{document}

\homework{13: Due 05/01}{There is hardly any theory which is more elementary [than linear algebra], in spite of the fact that generations of professors and textbook writers have obscured its simplicity by preposterous calculations with matrices.}{Jean Dieudonn\'e}

% Problem 1
\problem{10} Define $\mathbf{u}$, $\mathbf{v}$, and $\mathbf{w}$ to be the vectors given below:
	\[
	\mathbf{u}= \begin{pmatrix} 1 \\ -3 \\ 5 \end{pmatrix}, \qquad \mathbf{v}= \begin{pmatrix} 0 \\ 2 \\ -3 \end{pmatrix}, \qquad \mathbf{w}= \begin{pmatrix} 2 \\ -1 \\ 4 \end{pmatrix}
	\]
Compute the following:
	\begin{enumerate}[(a)]
	\item $-3 \mathbf{v}$
	\item $\mathbf{w} - \mathbf{u}$
	\item $2\mathbf{u} + \mathbf{v}$
	\item $\mathbf{v} \cdot \mathbf{w}$
	\end{enumerate} \pspace

\sol 
\begin{enumerate}[(a)]
\item 
	\[
	-3 \mathbf{v}= -3 \begin{pmatrix} 0 \\ 2 \\ -3 \end{pmatrix}= \begin{pmatrix} 0 \\ -6 \\ 9 \end{pmatrix}
	\] \pspace

\item 
	\[
	\mathbf{w} - \mathbf{u}= \begin{pmatrix} 2 \\ -1 \\ 4 \end{pmatrix} - \begin{pmatrix} 1 \\ -3 \\ 5 \end{pmatrix}= \begin{pmatrix} 2 - 1 \\ -1 - (-3) \\ 4 - 5 \end{pmatrix}= \begin{pmatrix} 1 \\ 2 \\ -1 \end{pmatrix}
	\] \pspace

\item 
	\[
	2\mathbf{u} + \mathbf{v}= 2 \begin{pmatrix} 1 \\ -3 \\ 5 \end{pmatrix} + \begin{pmatrix} 0 \\ 2 \\ -3 \end{pmatrix}= \begin{pmatrix} 2 \\ -6 \\ 10 \end{pmatrix} + \begin{pmatrix} 0 \\ 2 \\ -3 \end{pmatrix}= \begin{pmatrix} 2 + 0 \\ -6 + 2 \\ 10 + (-3) \end{pmatrix}= \begin{pmatrix} 2 \\ -4 \\ 7 \end{pmatrix}
	\] \pspace

\item 
	\[
	\mathbf{v} \cdot \mathbf{w}= \begin{pmatrix} 0 \\ 2 \\ -3 \end{pmatrix} \cdot \begin{pmatrix} 2 \\ -1 \\ 4 \end{pmatrix}= 0(2) + 2(-1) + (-3)4= 0 - 2 - 12= -14
	\]
\end{enumerate}



\newpage



% Problem 2
\problem{10} Define the following:
	\[
	A= \begin{pmatrix} 1 & 0 & -3 \\ 2 & -1 & 1 \\ 0 & 5 & 2 \end{pmatrix}, \qquad
	B= \begin{pmatrix} 2 & 1 & 1 \\ 0 & 3 & 0 \\ -1 & 4 & -2 \end{pmatrix}, \qquad
	\mathbf{u}= \begin{pmatrix} 1 \\ -1 \\ 1 \end{pmatrix}
	\]
Compute the following:
	\begin{enumerate}[(a)]
	\item $2B$
	\item $AB$
	\item $BA$
	\item $A \mathbf{u}$
	\end{enumerate} \pspace

\sol 
\begin{enumerate}[(a)]
\item 
	\[
	2B= 2 \begin{pmatrix} 2 & 1 & 1 \\ 0 & 3 & 0 \\ -1 & 4 & -2 \end{pmatrix}= \begin{pmatrix} 4 & 2 & 2 \\ 0 & 6 & 0 \\ -2 & 8 & -4 \end{pmatrix}
	\] \pspace

\item 
	\[
	\begin{aligned}
	AB&= \begin{pmatrix} 1 & 0 & -3 \\ 2 & -1 & 1 \\ 0 & 5 & 2 \end{pmatrix} \begin{pmatrix} 2 & 1 & 1 \\ 0 & 3 & 0 \\ -1 & 4 & -2 \end{pmatrix} \\[0.3cm]
	&= \begin{pmatrix} 1(2) + 0(0) + (-3)(-1) & 1(1) + 0(3) + (-3)4 & 1(1) + 0(1) + (-3)(-2) \\ 2(2) + (-1)0 + 1(-1) & 2(1) + (-1)3 + 1(4) & 2(1) + (-1)0 + 1(-2) \\ 0(2) + 5(0) + 2(-1) & 0(1) + 5(3) + 2(4) & 0(1) + 0(0) + 2(-2) \end{pmatrix} \\[0.3cm]
	&= \begin{pmatrix} 2 + 0 + 3 & 1 + 0 - 12 & 1 + 0 + 6 \\ 4 + 0 - 1 & 2 - 3 + 4 & 2 + 0 - 2 \\ 0 + 0 - 2 & 0 + 15 + 8 & 0 + 0 - 4 \end{pmatrix} \\[0.3cm]
	&= \begin{pmatrix} 5 & -11 & 7 \\ 3 & 3 & 0 \\ -2 & 23 & -4 \end{pmatrix}
	\end{aligned}
	\] \pspace

\item 
	\[
	\begin{aligned}
	BA&= \begin{pmatrix} 2 & 1 & 1 \\ 0 & 3 & 0 \\ -1 & 4 & -2 \end{pmatrix} \begin{pmatrix} 1 & 0 & -3 \\ 2 & -1 & 1 \\ 0 & 5 & 2 \end{pmatrix} \\[0.3cm]
	&= \begin{pmatrix} 2(1) + 1(2) + 1(0) & 2(0) + 1(-1) + 1(5) & 2(-3) + 1(1) + 1(2) \\ 0(1) + 3(2) + (-1)0 & 0(0) + 3(-1) + 0(5) & 0(-3) + 3(1) + 0(2) \\ (-1)1 + 4(2) + (-2)0 & -1(0) + 4(-1) + (-2)5 & -1(-3) + 4(1) + (-2)2 \end{pmatrix} \\[0.3cm]
	&= \begin{pmatrix} 2 + 2 + 0 & 0 - 1 + 5 & -6 + 1 + 2 \\ 0 + 6 + 0 & 0 - 3 + 0 & 0 + 3 + 0 \\ -1 + 8 + 0 & 0 - 4 - 10 & 3 + 4 - 4 \end{pmatrix} \\[0.3cm]
	&= \begin{pmatrix} 4 & 4 & -3 \\ 6 & -3 & 3 \\ 7 & -14 & 3 \end{pmatrix}
	\end{aligned}
	\] \pspace

\item 
	\[
	A\mathbf{u}= \begin{pmatrix} 1 & 0 & -3 \\ 2 & -1 & 1 \\ 0 & 5 & 2 \end{pmatrix} \begin{pmatrix} 1 \\ -1 \\ 1 \end{pmatrix}= \begin{pmatrix} 1(1) + 0(-1) + (-3)1 \\ 2(1) + (-1)(-1) + 1(1) \\ 0(1) + 5(-1) + 2(1) \end{pmatrix}= \begin{pmatrix} 1 + 0 - 3 \\ 2 + 1 + 1 \\ 0 - 5 + 2 \end{pmatrix}= \begin{pmatrix} -2 \\ 4 \\ -3 \end{pmatrix}
	\]
\end{enumerate}


\end{document}