\documentclass[12pt,letterpaper]{exam}
\usepackage[lmargin=1in,rmargin=1in,tmargin=1in,bmargin=1in]{geometry}
\usepackage{../style/exams}

% -------------------
% Course & Exam Information
% -------------------
\newcommand{\course}{MAT 101: Exam 2}
\newcommand{\term}{Spring -- 2022}
\newcommand{\examdate}{04/14/2022}
\newcommand{\timelimit}{85 Minutes}

\setbool{hideans}{false} % Student: True; Instructor: False

% -------------------
% Content
% -------------------
\begin{document}

\examtitle
\instructions{Write your name on the appropriate line on the exam cover sheet. This exam contains \numpages\ pages (including this cover page) and \numquestions\ questions. Check that you have every page of the exam. Answer the questions in the spaces provided on the question sheets. Be sure to answer every part of each question and show all your work.} 
\scores
%\bottomline
\newpage

% ---------
% Questions
% ---------
\begin{questions}

% Question 1
\newpage
\question[10] Sketch the quadratic function $f(x)= 8 - \left( x - \dfrac{13}{2} \right)^2$ on the plot below. Your sketch should include the vertex and axis of symmetry---being placed as accurately as possible. 
	\[
	\fbox{
	\begin{tikzpicture}[scale=2,every node/.style={scale=0.5}]
	\begin{axis}[
	grid=both,
	axis lines=middle,
	ticklabel style={fill=blue!5!white},
	xmin= -10.5, xmax=10.5,
	ymin= -10.5, ymax=10.5,
	xtick={-10,-8,-6,-4,-2,0,2,4,6,8,10},
	ytick={-10,-8,-6,-4,-2,0,2,4,6,8,10},
	minor tick = {-10,-9,...,10},
	xlabel=\(x\),ylabel=\(y\),
	]
	\draw[fill=black] (13/2,8) circle (0.15);
	\draw[line width=0.02cm,dotted] (13/2,-10.5) -- (13/2,10.5);
	\addplot[line width= 0.02cm,samples=100,domain= -10.5:10.5] ({x},{8 - (x- 13/2)^2}); 
	\end{axis}
	\end{tikzpicture}
	}
	\] \pspace

{\itshape We have $f(x)= 8 - \left( x - \dfrac{13}{2} \right)^2= - \left( x - \dfrac{13}{2} \right)^2 + 8$. Therefore, $f(x)$ is in vertex form, i.e. the form $f(x)= a(x - p)^2 + q$, where $(p, q)$ is the vertex. We then know that the vertex of $f(x)$ is $(-\frac{13}{2}, 8)$ so that the axis of symmetry is $x= \frac{13}{2}$. Because $a= -1 < 0$, the parabola opens downwards. This gives the sketch above.}



% Question 2
\newpage
\question Consider the quadratic function $y= (x + 5)^2 + 6$.

\begin{parts}
\part[2] Identify $a$, $b$, and $c$ for this quadratic function. \pvspace{0.3cm}

{\itshape
	\[
	y= (x + 5)^2 + 6= (x^2 + 10x + 25) + 6= x^2 + 10x + 31
	\] \pspace
Therefore, $a= 1$, $b= 10$, $c= 31$.} \pvspace{0.9cm}

\part[2] Does this quadratic function open upwards or downwards? \pvspace{1.6cm}

{\itshape Because $a= 1 > 0$, the quadratic function opens upwards.} \pvspace{1.6cm}

\part[2] Is this quadratic function convex or concave? \pvspace{1.6cm}

{\itshape Because $a= 1 > 0$, the quadratic function is convex} \pvspace{1.6cm}

\part[2] What is the vertex of this quadratic function? What is the axis of symmetry? \pvspace{1cm}

{\itshape The quadratic function $y= (x + 5)^2 + 6$ is in vertex form, i.e. $y= a(x - p)^2 + q$, where $(p, q)$ is the vertex. Therefore, the vertex is $(-5, 6)$ and the axis of symmetry is $x= -5$.} \pvspace{1cm}

\part[2] Find the maximum and minimum values for $y$. \pvspace{1cm}

{\itshape Because the parabola opens upwards, there is no maximum value, i.e. it does not exist. The parabola has a minimum. Because the vertex is $(-5, 6)$, we know the minimum value is 6---the $y$-coordinate of the vertex.}
\end{parts}



% Question 3
\newpage
\question[10] Find the vertex form of the quadratic function $f(x)= -3x^2 + 12x - 7$. \pspace

{\itshape Completing the square, we have\dots
	\[
	\begin{aligned}
	f(x)&= -3x^2 + 12x - 7 \\
	&= -3 \left( x^2 - 4x + \dfrac{7}{3} \right) \\
	&= -3 \left( x^2 - 4x + 4 - 4 + \dfrac{7}{3} \right) \\
	&= -3 \left( (x^2 - 4x + 4) - \dfrac{12}{3} + \dfrac{7}{3} \right) \\
	&= -3 \left( (x - 2)^2 - \dfrac{5}{3} \right) \\
	&= -3(x - 2)^2 + 5
	\end{aligned}
	\] \pspace
Alternatively, we can use the `evaluation method':
	\[
	\begin{aligned}
	a&= -3 \\
	x&= -\dfrac{b}{2a}= -\dfrac{12}{2(-3)}= -\dfrac{12}{-6}= -(-2)= 2 \\
	f(2)&= -3(2^2) + 12(2) - 7= -3(4) + 12(2) - 7= -12 + 24 - 7= 5
	\end{aligned}
	\]
This shows that the vertex, $(p, q)$, is $(2, 5)$. Therefore, the vertex form is\dots
	\[
	f(x)= a(x - p)^2 + q= -3(x - 2)^2 + 5
	\]
}



% Question 4
\newpage
\question[10] Factor $x^2 + 16x - 80$ completely. \pspace

{\itshape
	\begin{table}[!ht]
	\centering
	\underline{\bfseries 80} \pvspace{0.2cm}
	\begin{tabular}{rr}
	$1 \cdot -80$ & $-79$ \\
	$-1 \cdot 80$ & $79$ \\
	$2 \cdot -40$ & $-38$ \\
	$-2 \cdot 40$ & $38$ \\
	$4 \cdot -20$ & $-16$ \\ \hline
	\multicolumn{1}{|r}{$-4 \cdot 20$} & \multicolumn{1}{r|}{$16$} \\ \hline
	$5 \cdot -16$ & $-11$ \\
	$-5 \cdot 16$ & $11$ \\
	$8 \cdot -10$ & $-2$ \\
	$-8 \cdot 10$ & $2$
	\end{tabular}
	\end{table}

Therefore,
	\[
	x^2 + 16x - 80= (x - 4)(x + 20)
	\] 
}



% Question 5
\newpage
\question[10] Factor $3x^2 - 9x - 120$ completely. \pspace

{\itshape First, observe that $3x^2 - 9x - 120= 3(x^2 - 3x - 40)$. Then\dots
	\begin{table}[!ht]
	\centering
	\underline{\bfseries 40} \pvspace{0.2cm}
	\begin{tabular}{rr}
	$1 \cdot -40$ & $-39$ \\
	$-1 \cdot 40$ & $39$ \\
	$2 \cdot -20$ & $-18$ \\
	$-2 \cdot 20$ & $18$ \\
	$4 \cdot -10$ & $-6$ \\
	$-4 \cdot 10$ & $6$ \\ \hline
	\multicolumn{1}{|r}{$5 \cdot -8$} & \multicolumn{1}{r|}{$-3$} \\ \hline
	$-5 \cdot 8$ & $3$ 
	\end{tabular}
	\end{table}

Therefore,
	\[
	3x^2 - 9x - 120= 3(x^2 - 3x - 40)= 3(x + 5)(x - 8)
	\] 
}



% Question 6
\newpage
\question Factor the following completely: \pspace

\begin{parts}
\part[5] $16x - 20x^2$ \pvspace{1cm}

{\itshape Observe, we can factor out $4x$:
	\[
	16x - 20x^2= 4x(4 - 5x)
	\]
} \pvspace{6.85cm}

\part[5] $49 - x^2$ \pvspace{1cm}

{\itshape Observe that this is a difference of perfect squares:
	\[
	49 - x^2= (7 - x)(7 + x)
	\]
}
\end{parts}



% Question 7
\newpage
\question[10] Factor $10x^2 + 43x - 35$ completely. \pspace

{\itshape
	\begin{table}[!ht]
	\centering
	\underline{\bfseries 35} \pvspace{0.2cm}
	\begin{tabular}{cc}
	$1 \cdot -35$ \\
	$-1 \cdot 35$ \\
	$5 \cdot -7$ \\
	$-5 \cdot 7$
	\end{tabular}
	\end{table}

Then as $10= 1 \cdot 10$ or $10= 2 \cdot 5$, we have\dots
	\[
	\begin{tikzpicture}
	\node at (0,0) {$1 \cdot -35$};

	\node at (-1,0.5) {\footnotesize$1, 10$};
	\draw[line width=0.03cm,label={1}] (-0.2,0.3) -- (-0.8,1);
	\node at (-1,1.4) {$1, -350$};

	\node at (1,0.5) {\footnotesize$10, 1$};
	\draw[line width=0.03cm,label={1}] (0.2,0.3) -- (0.8,1);
	\node at (1,1.4) {$10, -35$};	
	
	\node at (-1,-0.5) {\footnotesize$2, 5$};
	\draw[line width=0.03cm,label={1}] (-0.2,-0.3) -- (-0.8,-1);
	\node at (-1,-1.4) {$2, -175$};

	\node at (1,-0.5) {\footnotesize$5, 2$};
	\draw[line width=0.03cm,label={1}] (0.2,-0.3) -- (0.8,-1);
	\node at (1,-1.4) {$5, -70$};

	\tikzset{shift={(7,0)}}
	
	\node at (0,0) {$-1 \cdot 35$};

	\node at (-1,0.5) {\footnotesize$1, 10$};
	\draw[line width=0.03cm,label={1}] (-0.2,0.3) -- (-0.8,1);
	\node at (-1,1.4) {$-1, 350$};

	\node at (1,0.5) {\footnotesize$10, 1$};
	\draw[line width=0.03cm,label={1}] (0.2,0.3) -- (0.8,1);
	\node at (1,1.4) {$-10, 35$};	
	
	\node at (-1,-0.5) {\footnotesize$2, 5$};
	\draw[line width=0.03cm,label={1}] (-0.2,-0.3) -- (-0.8,-1);
	\node at (-1,-1.4) {$-2, 175$};

	\node at (1,-0.5) {\footnotesize$5, 2$};
	\draw[line width=0.03cm,label={1}] (0.2,-0.3) -- (0.8,-1);
	\node at (1,-1.4) {$-5, 70$};
		
	\tikzset{shift={(-7,-4)}}
	
	\node at (0,0) {\framebox{$5 \cdot -7$}};

	\node at (-1,0.5) {\footnotesize$1, 10$};
	\draw[line width=0.03cm,label={1}] (-0.2,0.3) -- (-0.8,1);
	\node at (-1,1.4) {$5, -70$};

	\node at (1,0.5) {\footnotesize$10, 1$};
	\draw[line width=0.03cm,label={1}] (0.2,0.3) -- (0.8,1);
	\node at (1,1.4) {\framebox{$50, -7$}};	
	
	\node at (-1,-0.5) {\footnotesize$2, 5$};
	\draw[line width=0.03cm,label={1}] (-0.2,-0.3) -- (-0.8,-1);
	\node at (-1,-1.4) {$10, -35$};

	\node at (1,-0.5) {\footnotesize$5, 2$};
	\draw[line width=0.03cm,label={1}] (0.2,-0.3) -- (0.8,-1);
	\node at (1,-1.4) {$25, -14$};
	
	\tikzset{shift={(7,0)}}
	
	\node at (0,0) {$-5 \cdot 7$};

	\node at (-1,0.5) {\footnotesize$1, 10$};
	\draw[line width=0.03cm,label={1}] (-0.2,0.3) -- (-0.8,1);
	\node at (-1,1.4) {$-5, 70$};

	\node at (1,0.5) {\footnotesize$10, 1$};
	\draw[line width=0.03cm,label={1}] (0.2,0.3) -- (0.8,1);
	\node at (1,1.4) {$-50, 7$};	
	
	\node at (-1,-0.5) {\footnotesize$2, 5$};
	\draw[line width=0.03cm,label={1}] (-0.2,-0.3) -- (-0.8,-1);
	\node at (-1,-1.4) {$-10, 35$};

	\node at (1,-0.5) {\footnotesize$5, 2$};
	\draw[line width=0.03cm,label={1}] (0.2,-0.3) -- (0.8,-1);
	\node at (1,-1.4) {$-25, 14$};			
	\end{tikzpicture}
	\]

Therefore, 
	\[
	10x^2 + 43x - 35= (x + 5)(10x - 7)
	\] \pspace
Alternatively, we can use the quadratic formula to solve $10x^2 + 43x - 35= 0$:
	\[
	x= \dfrac{-b \pm \sqrt{b^2 - 4ac}}{2a}= \dfrac{-43 \pm \sqrt{43^2 - 4(10)(-35)}}{2(10)}= \dfrac{-43 \pm \sqrt{3249}}{20}= \dfrac{-43 \pm 57}{20}
	\]
This gives us $x= \frac{-43 - 57}{20}= -5$ and $x= \frac{-43 + 57}{20}= \frac{7}{10}$. Therefore, we know that $10x^2 + 43x - 35$ factors as\dots
	\[
	10x^2 + 43x - 35= a(x - r_1)(x - r_2)= 10(x + 5) \left( x - \frac{7}{10} \right)
	\]
We can see this is equivalent to the answer above via\dots
	\[
	10x^2 + 43x - 35= 10(x + 5) \left( x - \frac{7}{10} \right)= (x + 5) \cdot 10 \left( x - \frac{7}{10} \right)= (x + 5)(10x - 7)
	\]
}



% Question 8
\newpage
\question[10] Solve the following:
	\[
	5(6 - x)= \dfrac{4}{3}\,x + 30
	\] \pspace

	\[
	\begin{aligned}
	5(6 - x)&= \dfrac{4}{3}\,x + 30 \\[0.3cm]
	30 - 5x&= \dfrac{4}{3}\,x + 30 \\[0.3cm]
	-5x&= \dfrac{4}{3}\,x \\[0.3cm]
	-15x&= 4x \\[0.3cm]
	-19x&= 0 \\[0.3cm]
	x&= 0
	\end{aligned}
	\]



% Question 9
\newpage
\question[10] Solve the following:
	\[
	9= x(10 - x)
	\] \pspace

{\itshape
	\[
	\begin{aligned}
	9= x(10 - x) \\[0.3cm]
	9= 10x - x^2 \\[0.3cm]
	x^2 - 10x + 9= 0 \\[0.3cm]
	(x - 1)(x - 9)= 0
	\end{aligned}
	\] \pspace
But then either $x - 1=0$, so that $x= 1$, or $x - 9=0$, so that $x= 9$.}



% Question 10
\newpage
\question[10] Solve the following:
	\[
	6 - x= 12x + 7
	\] \pspace

	\[
	\begin{aligned}
	6 - x&= 12x + 7 \\[0.3cm]
	-1&= 13x \\[0.3cm]
	x&= -\dfrac{1}{13}
	\end{aligned}
	\] 



% Question 11
\newpage
\question[10] Solve the following:
	\[
	x(3x - 1)= x(x + 5)
	\] \pspace

{\itshape
	\[
	\begin{aligned}
	x(3x - 1)&= x(x + 5) \\[0.3cm]
	3x^2 - x&= x^2 + 5x \\[0.3cm]
	2x^2 - 6x&= 0 \\[0.3cm]
	2x(x - 3)&= 0
	\end{aligned}
	\] \pspace
But then either $2x= 0$, so that $x= 0$, or $x - 3=0$, so that $x= 3$. 
}



% Question 12
\newpage
\question[10] Solve the following:
	\[
	5(x + 5)= 4x^2 + 5x
	\] \pspace

{\itshape
	\[
	\begin{aligned}
	5(x + 5)=& 4x^2 + 5x \\[0.3cm]
	5x + 25=& 4x^2 + 5x \\[0.3cm]
	25= & \;4x^2 \\[0.3cm]
	0= 4x^2 &- 25 \\[0.3cm]
	0= (2x - 5)&(2x + 5)
	\end{aligned}
	\] \pspace
But then either $2x - 5= 0$, which implies $x= \dfrac{5}{2}$, or $2x + 5= 0$, which implies that $x= -\dfrac{5}{2}$. \pspace

Alternatively, we have
	\[
	\begin{aligned}
	5(x + 5)=& 4x^2 + 5x \\[0.3cm]
	5x + 25=& 4x^2 + 5x \\[0.3cm]
	25= & \;4x^2 \\[0.3cm]
	x^2&= \dfrac{25}{4} \\[0.3cm]
	x&= \pm \sqrt{\dfrac{25}{4}} \\[0.3cm]
	x&= \pm \dfrac{5}{2}
	\end{aligned}
	\] 
Therefore, $x= -\frac{5}{2}$ or $x= \frac{5}{2}$. 
}



% Question 13
\newpage
\question[10] Use the quadratic formula to solve the following:
	\[
	6 - 5x^2= 4x(1 - x)
	\] \pspace

{\itshape We have\dots
	\[
	\begin{aligned}
	6 - 5x^2= 4x(1 - x) \\[0.3cm]
	6 - 5x^2= 4x - 4x^2 \\[0.3cm]
	x^2 + 4x - 6= 0 
	\end{aligned}
	\] \pspace
But then we have\dots
	\[
	\begin{aligned}
	x&= \dfrac{-b \pm \sqrt{b^2 - 4ac}}{2a} \\[0.3cm]
	&=  \dfrac{-4 \pm \sqrt{4^2 - 4(1)(-6)}}{2(1)} \\[0.3cm]
	&=  \dfrac{-4 \pm \sqrt{16 + 24}}{2} \\[0.3cm]
	&= \dfrac{-4 \pm \sqrt{40}}{2} \\[0.3cm]
	&= \dfrac{-4 \pm \sqrt{4 \cdot 10}}{2} \\[0.3cm]
	&= \dfrac{-4 \pm 2\sqrt{10}}{2} \\[0.3cm]
	&= -2 \pm \sqrt{10}
	\end{aligned}
	\] \pspace
Therefore, the solutions are $x= -2 - \sqrt{10}$ and $x= -2 + \sqrt{10}$. 
}



% Question 14
\newpage
\question[10] Use the quadratic formula to factor $x^2 - 10x + 23$. \pspace

{\itshape We find the roots of $x^2 - 10x + 23$ using the quadratic formula: \pspace
	\[
	\begin{aligned}
	x&= \dfrac{-b \pm \sqrt{b^2 - 4ac}}{2a} \\[0.3cm]
	&=  \dfrac{-(-10) \pm \sqrt{(-10)^2 - 4(1)(23)}}{2(1)} \\[0.3cm]
	&= \dfrac{10 \pm \sqrt{100 - 92}}{2} \\[0.3cm]
	&= \dfrac{10 \pm \sqrt{8}}{2} \\[0.3cm]
	&= \dfrac{10 \pm \sqrt{4 \cdot 2}}{2} \\[0.3cm]
	&= \dfrac{10 \pm 2\sqrt{2}}{2} \\[0.3cm]
	&= 5 \pm \sqrt{2}
	\end{aligned}
	\] \pspace
Therefore, the roots are $r_1= 5 - \sqrt{2}$ and $r_2= 5 + \sqrt{2}$. Using the fact that $a= 1$, we then know that $x^2 - 10x + 23$ factors as\dots \pspace
	\[
	x^2 - 10x + 23= a(x - r_1)(x - r_2)= 1 \big(x - (5 - \sqrt{2}) \big)  \big(x - (5 + \sqrt{2}) \big)=  \big(x - (5 - \sqrt{2}) \big)  \big(x - (5 + \sqrt{2}) \big)
	\]
}



% Question 15
\newpage
\question[10] Use the discriminant to determine whether the function $384x^2 + 232x - 175$ factors `nicely', i.e. over the integers. If not, determine whether it even factors over the real numbers or requires complex numbers to factor. \pspace

{\itshape
	\[
	\begin{aligned}
	D&= b^2 - 4ac \\[0.3cm]
	&= 232^2 - 4(384)(-175) \\[0.3cm]
	&= 53824 + 268800 \\[0.3cm]
	&= 322624 \\[0.3cm]
	&= 568^2
	\end{aligned}
	\] \pspace
Because the discriminant is a perfect square, the function $384x^2 + 232x - 175$ factors `nicely', i.e. over the integers. Therefore, $384x^2 + 232x - 175$ also factors `nicely' over the rational numbers, real numbers, and complex numbers. 
}



% Question 16
\newpage
\question[10] Showing all your work, determine if the point $(5, -4)$ is a solution to the following system of equations:
	\[
	\begin{aligned}
	2x + y&= 6 \\[0.3cm]
	-5x - 6y&= -49
	\end{aligned}
	\] \pspace

{\itshape The point $(x, y)= (5, -4)$ is a solution to the system of equations if and only if it satisfies both of the equations. We check this:
	\[
	\begin{aligned}
	2x + y&= 6 \\[0.3cm]
	2(5) + (-4)&\stackrel{?}{=} 6 \\[0.3cm]
	10 - 4&\stackrel{?}{=} 6 \\[0.3cm]
	6&= 6 \\
	&\;\,\text{\cmark}
	\end{aligned}
	\]
and
	\[
	\begin{aligned}
	-5x - 6y&= -49 \\[0.3cm]
	-5(5) - 6(-4)&\stackrel{?}{=} -49 \\[0.3cm]
	-25 + 24&\stackrel{?}{=} -49 \\[0.3cm]
	-1&\neq -49 \\
	&\;\,\text{\xmark}
	\end{aligned}
	\] \pspace
Because $(5, -4)$ does not satisfy both of the equations, $(x, y)= (5, -4)$ is not a solution to the system of equations. [Indeed, there is no solution to this system of equations because the given lines are parallel.]
}



% Question 17
\newpage
\question[10] Showing all your work, determine whether the following system of equations has a solution. If it has a solution, you do not need to find the solution.
	\[
	\begin{aligned}
	10x - 4y&= -24 \\[0.3cm]
	-5x + 2y&= -2
	\end{aligned}
	\] \pspace

{\itshape Solving for $y$ in both equations, we have\dots
	\[
	\begin{aligned}
	10x - 4y&= -24 \\[0.3cm]
	-4y&= -10x - 24 \\[0.3cm]
	y&= \dfrac{5}{2}\,x + 6
	\end{aligned}
	\] 
and
	\[
	\begin{aligned}
	-5x + 2y&= -2 \\[0.3cm]
	2y&= 5x - 2 \\[0.3cm]
	y&= \dfrac{5}{2}\,x - 1
	\end{aligned}
	\] \pspace
Both lines have slope $\frac{5}{2}$. But then the lines are parallel so that they do not interest. Because there cannot be a point on both the lines at once, there are no solutions to the given system of equations.
}



% Question 18
\newpage
\question[10] Solve the following system of equations:
	\[
	\begin{aligned}
	3x + 5y&= 16 \\[0.3cm]
	x + 6y&= 1
	\end{aligned}
	\] \pspace

{\itshape Using substitution, from the second equation, we have\dots
	\[
	\begin{aligned}
	x + 6y&= 1 \\[0.3cm]
	x&= 1 - 6y
	\end{aligned}
	\]
Using this in the first equation, we have\dots
	\[
	\begin{aligned}
	3x + 5y&= 16 \\[0.3cm]
	3(1 - 6y) + 5y&= 16 \\[0.3cm]
	3 - 18y + 5y&= 16 \\[0.3cm]
	3 - 13y&= 16 \\[0.3cm]
	-13y&= 13 \\[0.3cm]
	y&= -1
	\end{aligned}
	\]
Then we have $x= 1 - 6y= 1 - 6(-1)= 1 + 6= 7$. Therefore, the solution is $(7, -1)$. 

	\begin{center} {\bfseries OR} \end{center}

Using elimination, we multiply the second equation by $-3$. This yields\dots
	\[
	\begin{aligned}
	3x + 5y&= 16 \\[0.3cm]
	-3x - 18y&= -3 
	\end{aligned}
	\]
Adding these equations, we have\dots
	\[
	\begin{aligned}
	-13y&= 13 \\[0.3cm]
	y&= -1
	\end{aligned}
	\]
Using this in the second equation, we have $x + 6y= 1$ so that $x + 6(-1)= 1$. But then $x - 6= 1$. Therefore, $x= 7$. The solution is then $(7, -1)$. 
}



% Question 19
\newpage
\question[10] Solve the following system of equations:
	\[
	\begin{aligned}
	4x + 7y&= -8 \\[0.3cm]
	2x - 5y&= -4
	\end{aligned}
	\]

{\itshape Using substitution, from the first equation, we have\dots
	\[
	\begin{aligned}
	4x + 7y&= -8 \\[0.3cm]
	7y&= -4x - 8 \\[0.3cm]
	y&= -\dfrac{4}{7}\,x - \dfrac{8}{7}
	\end{aligned}
	\]
Using this in the second equation, we have\dots
	\[
	\begin{aligned}
	2x - 5y&= -4 \\[0.3cm]
	2x - 5 \left( -\dfrac{4}{7}\,x - \dfrac{8}{7} \right)&= -4 \\[0.3cm]
	2x + \dfrac{20}{7}\,x + \dfrac{40}{7}&= -4 \\[0.3cm]
	7 \left( 2x + \dfrac{20}{7}\,x + \dfrac{40}{7} \right)&= -4 \cdot 7 \\[0.3cm]
	14x + 20x + 40&= -28 \\[0.3cm]
	34x + 40&= -28 \\[0.3cm]
	34x&= -68 \\[0.3cm]
	x&= -2
	\end{aligned}
	\]
Then we have $y= -\frac{4}{7} \cdot -2 - \frac{8}{7}= \frac{8}{7} - \frac{8}{7}= 0$. Therefore, the solution is $(-2, 0)$. 

	\begin{center} {\bfseries OR} \end{center}

Using elimination, we multiply the second equation by $-2$. This yields\dots
	\[
	\begin{aligned}
	4x + 7y&= -8 \\[0.3cm]
	-4x + 10y&= 8
	\end{aligned}
	\]
Adding these equations, we have\dots
	\[
	\begin{aligned}
	17y&= 0 \\
	y&= 0
	\end{aligned}
	\]
Using this in the first equation, we have $4x + 7y= -8$ so that $4x + 7(0)= -8$. But then $4x= -8$. Therefore, $x= -2$. The solution is then $(-2, 0)$. 
}



% Question 20
\newpage
\question[10] A quadratic function $y= x^2 - 2x + 1$ and a linear function $y= x + 1$ are plotted below.
	\[
	\fbox{
	\begin{tikzpicture}[scale=1.5,every node/.style={scale=0.5}]
	\begin{axis}[
	grid=both,
	axis lines=middle,
	ticklabel style={fill=blue!5!white},
	xmin= -6.5, xmax=6.5,
	ymin= -6.5, ymax=6.5,
	xtick={-6,-4,-2,0,2,4,6},
	ytick={-6,-4,-2,0,2,4,6},
	minor tick = {-7,-6,...,7},
	xlabel=\(x\),ylabel=\(y\),
	]
	\addplot[line width= 0.02cm,samples=100,domain= -10.5:10.5] ({x},{x^2 - 2*x + 1}); 
	\addplot[line width= 0.02cm,samples=100,domain= -10.5:10.5] ({x},{x + 1}); 
	\end{axis}
	\end{tikzpicture}
	}
	\] \pspace

\begin{parts}
\part[5] Using the plot above, solve the following system of equations:
	\[
	\begin{aligned}
	-x + y&= 1 \\
	2x + y&= x^2 + 1
	\end{aligned}
	\] 

{\itshape The first equation is equivalent to $y= x + 1$ and the second is equivalent to $y= x^2 - 2x + 1$. Solving the system of equations is then equivalent to finding the intersection points between these curves, i.e. the parabola and the line. From the plot above, we see the solutions are $(x, y)= (0, 1)$ and $(x, y)= (3, 4)$.} \pvspace{0.75cm}

\part[5] Setting the functions equal, verify the solution(s) to the system of equations from (a). \pspace

{\itshape We have\dots
	\[
	\begin{aligned}
	x^2 - 2x + 1&= x + 1 \\
	x^2 - 3x&= 0 \\
	x(x - 3)&= 0
	\end{aligned}
	\]
But then either $x= 0$ or $x - 3= 0$, so that $x= 3$. Using the fact that $y= x + 1$, we see that if $x= 0$, $y= 0 + 1= 1$. If $x= 3$, $y= 3 + 1= 4$. Therefore, the solutions are $(0, 1)$ and $(3, 4)$, which is what we obtained in (a).
}
\end{parts}


\end{questions}
\end{document}