\documentclass[11pt,letterpaper]{article}
\usepackage[lmargin=1in,rmargin=1in,tmargin=1in,bmargin=1in]{geometry}
\usepackage{../style/homework}
\usepackage{../style/commands}
\setbool{quotetype}{true} % True: Side; False: Under
\setbool{hideans}{false} % Student: True; Instructor: False

% -------------------
% Content
% -------------------
\begin{document}

\homework{14: Due 12/08}{One morning I shot an elephant in my pajamas. How he got into my pajamas I'll never know.}{Groucho Marx}

% Problem 1
\problem{10} Solve the following system of equations using substitution:
	\[
	\begin{aligned}
	y= 2x - 3 \\
	3x - y= 4
	\end{aligned}
	\] \pspace

\sol The first equation is already expressed in terms of $y$. Using this expression for $y$ in the second equation, we have\dots
	\[
	\begin{aligned}
	3x - y&= 4 \\[0.3cm]
	3x - (2x - 3)&= 4 \\[0.3cm]
	3x - 2x + 3&= 4 \\[0.3cm]
	x + 3&= 4 \\[0.3cm]
	x&= 1
	\end{aligned}
	\] 
But then we know that $y= 2(1) - 3= 2 - 3= -1$. Therefore, the solution is $(1, -1)$. 





\newpage





% Problem 2
\problem{10} Solve the following system of equations using substitution: 
	\[
	\begin{aligned}
	2x - 3y&= -12 \\
	3x + 5y&= 1
	\end{aligned}
	\] \pspace

\sol We solve for $y$ in the first equation:
	\[
	\begin{aligned}
	2x - 3y&= -12 \\[0.3cm]
	-3y&= -2x - 12 \\[0.3cm]
	y&= \frac{2}{3}\,x + 4
	\end{aligned}
	\]
Using this expression in the second equation, we have\dots
	\[
	\begin{aligned}
	3x + 5y&= 1 \\[0.3cm]
	3x + 5\left(\frac{2}{3}\,x + 4 \right)&= 1 \\[0.3cm]
	3x + \frac{10}{3}\, x + 20&= 1 \\[0.3cm]
	3 \left( 3x + \frac{10}{3}\, x + 20 \right)&= 1 \cdot 3 \\[0.3cm]
	9x + 10x + 60&= 3 \\[0.3cm]
	19x + 60&= 3 \\[0.3cm]
	19x&= -57 \\[0.3cm]
	x&= -3
	\end{aligned}
	\]
But then $y= \frac{2}{3} \cdot -3 + 4= -2 + 4= 2$. Therefore, the solution is $(-3, 2)$. 





\newpage





% Problem 3
\problem{10} Solving the following system of equations using elimination: 
	\[
	\begin{aligned}
	x - 3y&= 5 \\ 
	-x + 5y&= 7
	\end{aligned}
	\] \pspace

\sol We add the equations to immediately eliminate the $x$-term:
	\[
	\begin{aligned}
	x - 3y&= 5 \\ 
	-x + 5y&= 7 \\ \hline
	2y&= 12 \\
	y&= 6
	\end{aligned}
	\] 
But then we know that\dots
	\[
	\begin{aligned}
	x - 3y&= 5 \\[0.3cm]
	x - 3(6)&= 5 \\[0.3cm]
	x - 18&= 5 \\[0.3cm]
	x&= 23
	\end{aligned}
	\] 
Therefore, the solution is $(23, 6)$. 





\newpage





% Problem 4
\problem{10} Solving the following system of equations using elimination:  
	\[
	\begin{aligned}
	2x - 3y&= 17 \\
	3x + 2y&= 6
	\end{aligned}
	\] \pspace

\sol We eliminate the $y$ terms. Multiplying the first equation by 2 and the second equation by 3, we have\dots
	\[
	\begin{aligned}
	4x - 6y&= 34 \\
	9x + 6y&= 18
	\end{aligned}
	\] 
Then we add these equations to find\dots
	\[
	\begin{aligned}
	4x - 6y&= 34 \\
	9x + 6y&= 18 \\ \hline
	13x&= 52 \\
	x&= 4
	\end{aligned}
	\] 
But then we have\dots
	\[
	\begin{aligned}
	4x - 6y&= 34 \\[0.3cm]
	4(4) - 6y&= 34 \\[0.3cm]
	16 - 6y&= 34 \\[0.3cm]
	-6y&= 18 \\[0.3cm]
	y&= -3
	\end{aligned}
	\] 
Therefore, the solution is $(4, -3)$. 


%\printpoints
\end{document}