\documentclass[11pt,letterpaper]{article}
\usepackage[lmargin=1in,rmargin=1in,tmargin=1in,bmargin=1in]{geometry}
\usepackage{../style/homework}
\setbool{quotetype}{false} % True: Side; False: Under
\setbool{hideans}{false} % Student: True; Instructor: False

% -------------------
% Content
% -------------------
\begin{document}

\homework{4: Due 02/05}{Now we're going to do the most human thing of all: attempt something futile with a ton of unearned confidence and fail spectacularly!}{Michael, The Good Place}

% Problem 1
\problem{10} Showing all your work, compute the following ``without a calculator'': 
	\begin{enumerate}[(a)]
	\item $\sqrt[3]{64}$
	\item $36^{-3/2}$
	\item $\left( \dfrac{1}{8} \right)^{-1/3}$
	\end{enumerate} \pspace

\sol 
\begin{enumerate}[(a)]
\item 
	\[
	\sqrt[4]{64}= \sqrt[4]{2^6}= 2^1 \sqrt[4]{2^2}= 2 \sqrt[4]{4} \quad \big(= 2 \cdot 4^{1/4}= 2 \cdot (2^2)^{1/4}= 2 \cdot 2^{2/4}= 2 \cdot 2^{1/2}= 2 \sqrt{2} \big)
	\] \pspace

\item 
	\[
	36^{-3/2}= \big(36^{1/2} \big)^{-3}= \big( \sqrt{36} \big)^{-3}= 6^{-3}= \dfrac{1}{6^3}= \dfrac{1}{216}
	\] \pspace

\item 
	\[
	\left( \dfrac{1}{8} \right)^{-1/3}= \left( \dfrac{8}{1} \right)^{1/3}= 8^{1/3}= \sqrt[3]{8}= \sqrt[3]{2^3}= 2^1 \sqrt[3]{2^0}= 2 \cdot 1= 2
	\]
\end{enumerate}



\newpage



% Problem 2
\problem{10} Simplify the following:
	\begin{enumerate}[(a)]
	\item $\sqrt{x^{10} y^4}$
	\item $\sqrt[3]{x^3 y^5 z^{12}}$
	\item $\sqrt{\sqrt[3]{y^6}}$
	\end{enumerate} \pspace

\sol 
\begin{enumerate}[(a)]
\item 
	\[
	\sqrt{x^{10} y^4}= x^5 y^2 \sqrt{x^0 y^0}= x^5 y^2
	\] \pspace

\item 
	\[
	\sqrt[3]{x^3 y^5 z^{12}}= x^1 y^1 z^4 \sqrt[3]{x^0 y^2 z^0}= x y z^4 \sqrt[3]{y^2}
	\] \pspace

\item 
	\[
	\sqrt{\sqrt[3]{y^6}}= \left( \big( y^6 \big)^{1/3} \right)^{1/2}= \big(y^6 \big)^{1/6}= \sqrt[6]{y^6}= y^1 \sqrt[6]{y^0}= y
	\]
\end{enumerate}



\newpage



% Problem 3
\problem{10} Simplify the following:
	\begin{enumerate}[(a)]
	\item $x^2 y \sqrt{x^8 y^5}$
	\item $\dfrac{x^2 y}{\sqrt[3]{x y^6}}$
	\item $\dfrac{\sqrt{x^2 y}}{\sqrt[3]{x^3 y^5}}$
	\end{enumerate} \pspace

\sol 
\begin{enumerate}[(a)]
\item 
	\[
	x^2 y \sqrt{x^8 y^5}= x^2 y \cdot x^4 y^2 \sqrt{x^0 y^1}= x^2 y \cdot x^4 y^2 \sqrt{y}= x^6 y^3 \sqrt{y}
	\] \pspace

\item 
	\[
	\dfrac{x^2 y}{\sqrt[3]{x y^6}}= \dfrac{x^2 y}{y^2 \sqrt[3]{x y^0}}= \dfrac{x^2 y}{y^2 \sqrt[3]{x}}= \dfrac{x^2}{y^2 \sqrt[3]{x}}= \dfrac{x^2}{y^2 x^{1/3}}= \dfrac{x^{2 - \frac{1}{3}}}{y^2}= \dfrac{x^{5/3}}{y^2}= \dfrac{\sqrt[3]{x^5}}{y^2}
	\] \pspace

\item 
	\[
	\dfrac{\sqrt{x^2 y}}{\sqrt[3]{x^3 y^5}}= \dfrac{x^{2/2} y^{1/2}}{x^{3/3} y^{5/3}}= \dfrac{x y^{1/2}}{x^1 y^{5/3}}= \dfrac{y^{1/2}}{y^{5/3}}= y^{\frac{1}{2} - \frac{5}{3}}= y^{-7/6}= \dfrac{1}{y^{7/6}}= \dfrac{1}{\sqrt[6]{y^7}}
	\] 
\end{enumerate}



\newpage



% Problem 4
\problem{10} Simplify the following:
	\[
	\left( \dfrac{\sqrt{x^8 y^6}}{x^{-3} \sqrt{x y}} \right)^{-3/2}
	\] \pspace

\sol 
	\[
	\begin{gathered}
	\left( \dfrac{\sqrt{x^8 y^6}}{x^{-3} \sqrt{x y}} \right)^{-3/2} \\[0.3cm]
	\left( \dfrac{x^{8/2} y^{6/2}}{x^{-3} x^{1/2} y^{1/2}} \right)^{-3/2} \\[0.3cm]
	\left( \dfrac{x^4 y^3}{x^{-3 + \frac{1}{2}} y^{1/2}} \right)^{-3/2} \\[0.3cm]
	\left( \dfrac{x^4 y^3}{x^{-5/2} y^{1/2}} \right)^{-3/2} \\[0.3cm]
	\left( \dfrac{x^4 x^{5/2} y^3}{y^{1/2}} \right)^{-3/2} \\[0.3cm]
	\left( x^{4 + \frac{5}{2}} y^{3 - \frac{1}{2}} \right)^{-3/2} \\[0.3cm]
	\left( x^{13/2} y^{5/2} \right)^{-3/2} \\[0.3cm]
	x^{-39/4} y^{-15/4} \\[0.3cm]
	\dfrac{1}{x^{39/4} y^{15/4}} \\[0.3cm]
	\dfrac{1}{\sqrt[4]{x^{39} y^{15}}}
	\end{gathered}
	\]


\end{document}