\documentclass[11pt,letterpaper]{article}
\usepackage[lmargin=1in,rmargin=1in,tmargin=1in,bmargin=1in]{geometry}
\usepackage{../style/homework}
\usepackage{../style/commands}
\setbool{quotetype}{false} % True: Side; False: Under
\setbool{hideans}{false} % Student: True; Instructor: False

% -------------------
% Content
% -------------------
\begin{document}

\homework{2: Due 05/25}{Sometimes the questions are complicated and the answers are simple.}{Dr. Seuss (Theodor Seuss Geisel)}

% Problem 1
\problem{10} Is the following statement true or false, explain: for a nonzero real number $x$ and integer $n$, $x^n= \dfrac{1}{x^{-n}}$. \pspace

\sol The statement is true. Observe that if $x \neq 0$ is a real number and $n$ is an integer, then we have\dots
	\[
	\dfrac{1}{x^{-n}}= \dfrac{1}{1/x^n}= \dfrac{1}{1} \cdot \dfrac{x^n}{1}= x^n
	\]



\newpage



% Problem 2
\problem{10} Write the following complex numbers in the form $a + bi$:
	\begin{enumerate}[(a)]
	\item $2(1 - 3i) - (6 - 4i)$
	\item $(3 + 4i)(2 - i)$
	\item $(2i)^5$
	\item $\dfrac{5 - i}{1 + 2i}$
	\end{enumerate} \pspace

\sol
\begin{enumerate}[(a)]
\item 
	\[
	2(1 - 3i) - (6 - 4i)= (2 - 6i) - (6 - 4i)= 2 - 6i - 6 + 4i= -4 - 2i
	\] \pspace

\item 
	\[
	(3 + 4i)(2 - i)= 6 - 3i + 8i - 4i^2= 6 - 3i + 8i - 4(-1)= 6 - 3i + 8i + 4= 10 + 5i
	\] \pspace

\item 
	\[
	(2i)^5= 2^5 \cdot i^5= 2^5 \cdot (i^4 \cdot i)= 32 \cdot (1 \cdot i)= 32i 
	\] \pspace

\item 
	\[
	\dfrac{5 - i}{1 + 2i}= \dfrac{5 - i}{1 + 2i} \cdot \dfrac{1 - 2i}{1 - 2i}= \dfrac{5 - 10i - i + 2i^2}{1 - 2i + 2i - 4i^2}= \dfrac{5 - 11i - 2}{1 - 4(-1)}= \dfrac{3 - 11i}{5}= \tfrac{3}{5} - \tfrac{11}{5}\, i
	\]
\end{enumerate}



\newpage



% Problem 3
\problem{10} Write the following numbers in scientific notation as a decimal value:
	\begin{enumerate}[(a)]
	\item $5.77 \cdot 10^5$
	\item $-1.41 \cdot 10^{-2}$
	\item $8.9 \cdot 10^0$
	\item $4.5 \cdot 10^{-6}$
	\end{enumerate} \pspace

\sol
\begin{enumerate}[(a)]
\item $5.77 \cdot 10^5= 577\,000$

\item $-1.41 \cdot 10^{-2}= -0.0141$

\item $8.9 \cdot 10^0= 8.9$

\item $4.5 \cdot 10^{-6}= 0.0000045$
\end{enumerate}



\newpage



% Problem 4
\problem{10} Write the following decimal numbers in scientific notation:
	\begin{enumerate}[(a)]
	\item $34100000$
	\item $7.7$
	\item $0.6631$
	\item $0.0000004$
	\end{enumerate} \pspace

\sol
\begin{enumerate}[(a)]
\item $34100000= 3.41 \cdot 10^7$
\item $7.7= 7.7 \cdot 10^0$
\item $0.6631= 6.631 \cdot 10^{-1}$
\item $0.0000004= 4.0 \cdot 10^{-7}$
\end{enumerate}



\newpage



% Problem 5
\problem{10} Using no negative powers and showing all your work, simplify the following:
	\begin{enumerate}[(a)]
	\item $(x^5 y^3)^2 (x^{10} y^2)^0$
	\item $x^3 (x^2y)^2 y^3$
	\item $x^3 y^8(x^5 y^2)^{-2}$
	\item $(xy^4)^{-3} (x^5 y^{-3})^{-5}$
	\end{enumerate} \pspace

\sol
\begin{enumerate}[(a)]
\item 
	\[
	(x^5 y^3)^2 (x^{10} y^2)^0= (x^{5 \cdot 2} y^{3 \cdot 2}) \cdot 1= x^{10} y^6
	\] \pspace

\item 
	\[
	x^3 (x^2y)^2 y^3= x^3 \cdot x^4 y^2 \cdot y^3= x^{3 + 4} y^{2 + 3}= x^7 y^5
	\] \pspace

\item 
	\[
	x^3 y^8(x^5 y^2)^{-2}= \dfrac{x^3 y^8}{(x^5 y^2)^2}= \dfrac{x^3 y^8}{x^{10} y^4}= \dfrac{\cancel{x^3} y^{\cancel{8}^4}}{x^{\cancel{10}^7} \cancel{y^4}}= \dfrac{y^4}{x^7}
	\] \pspace

\item 
	\[
	(xy^4)^{-3} (x^5 y^{-3})^{-5}= x^{-3} y^{-12} \cdot x^{-25} y^{15}= x^{-3 - 25} y^{-12 + 15}= x^{-28} y^3= \dfrac{y^3}{x^{28}}
	\]
\end{enumerate}



\newpage



% Problem 6
\problem{10} Using no negative powers and showing all your work, simplify the following:
        \begin{enumerate}[(a)]
        \item $\dfrac{x^5 y^7}{x^4 y^{12}}$
        \item $\dfrac{x^8 y^{-3}}{x^{12} y^{-6}}$
        \item $\dfrac{(xy^3)^{-2}}{x^{-5} y^2}$
        \item $\dfrac{x^3 (x^2y)^0}{y^5(xy^3)^{-2}}$
        \end{enumerate} \pspace

\sol
\begin{enumerate}[(a)]
\item 
	\[
	\dfrac{x^5 y^7}{x^4 y^{12}}= x^{5 - 4} y^{7 - 12}= x^1 y^{-5}= \dfrac{x}{y^5}
	\] \pspace

\item 
	\[
	\dfrac{x^8 y^{-3}}{x^{12} y^{-6}}= \dfrac{x^8 y^6}{x^{12} y^3}= \dfrac{y^3}{x^4}
	\] \pspace

\item 
	\[
	\dfrac{(xy^3)^{-2}}{x^{-5} y^2}= \dfrac{x^5}{(x y^3)^2 y^2}= \dfrac{x^5}{x^2 y^6 y^2}= \dfrac{x^5}{x^2 y^8}= \dfrac{x^3}{y^8}
	\] \pspace

\item 
	\[
	\dfrac{x^3 (x^2y)^0}{y^5(xy^3)^{-2}}= \dfrac{x^3 \cdot 1 \cdot (xy^3)^2}{y^5}= \dfrac{x^3 \cdot x^2 y^6}{y^5}= \dfrac{x^5 y^6}{y^5}= x^5y
	\]
\end{enumerate}



\newpage



% Problem 7
\problem{10} Using no negative powers, being sure each variable appears only once, and showing all your work, simplify the following:
        \begin{enumerate}[(a)]
        \item $xy\sqrt{x^5y^3}$
        \item $\dfrac{y \sqrt{x^5}}{\sqrt{x^3y}}$
        \item $\dfrac{(x^2 y^5)^{1/2}}{(x^6 y^{2})^{-1/3}}$
        \item $(x^{10} y^{-4})^{-1/4} \sqrt{xy}$
        \end{enumerate} \pspace

\sol
\begin{enumerate}[(a)]
\item 
	\[
	xy\sqrt{x^5y^3}= xy (x^5 y^3)^{1/2}= xy \cdot x^{5/2} y^{3/2}= x^{1 + 5/2} y^{1 + 3/2}= x^{7/2} y^{5/2}= \sqrt{x^7 y^5}
	\] \pspace

\item 
	\[
	\dfrac{y \sqrt{x^5}}{\sqrt{x^3y}}= \dfrac{y x^{5/2}}{(x^3 y)^{1/2}}= \dfrac{y x^{5/2}}{x^{3/2} y^{1/2}}= x^{5/2 - 3/2} y^{1 - 1/2}= x y^{1/2}= x \sqrt{y}
	\] \pspace

\item 
	\[
	\dfrac{(x^2 y^5)^{1/2}}{(x^6 y^{2})^{-1/3}}= (x^{2/2} y^{5/2}) \cdot (x^6 y^2)^{1/3}= xy^{5/2} \cdot x^2 y^{2/3}= x^{1 + 2} y^{5/2 + 2/3}= x^3 y^{19/6}= x^3 \sqrt[6]{y^{19}}
	\] \pspace

\item 
	\[
	(x^{10} y^{-4})^{-1/4} \sqrt{xy}= x^{-10/4} y^{4/4} \cdot (xy)^{1/2}= x^{-5/2} y \cdot x^{1/2} y^{1/2}= x^{-5/2 + 1/2} y^{1 + 1/2}= x^{-2} y^{3/2}= \dfrac{\sqrt{y^3}}{x^2}
	\] 
\end{enumerate}



\newpage



% Problem 8
\problem{10} Showing all your work, simplify the following as much as possible:
        \begin{enumerate}[(a)]
        \item $\sqrt{75}$
        \item $\sqrt{250}$
        \item $\sqrt{360}$
        \item $\sqrt{2^7 \cdot 3^3 \cdot 5^2 \cdot 11}$
        \end{enumerate} \pspace

\sol
\begin{enumerate}[(a)]
\item 
	\[
	\sqrt{75}= \sqrt{3 \cdot 5^2}= 5 \sqrt{3}
	\] \pspace

\item 
	\[
	\sqrt{250}= \sqrt{2 \cdot 5^3}= \sqrt{2 \cdot (5^2 \cdot 5)}= 5 \sqrt{2 \cdot 5}= 5 \sqrt{10}
	\] \pspace

\item 
	\[
	\sqrt{360}= \sqrt{2^3 \cdot 3^2 \cdot 5}= \sqrt{(2^2 \cdot 2) \cdot 3^2 \cdot 5}= 2 \cdot 3 \sqrt{2 \cdot 5}= 6 \sqrt{10}
	\] \pspace

\item 
	\[
	\sqrt{2^7 \cdot 3^3 \cdot 5^2 \cdot 11}= \sqrt{(2^6 \cdot 2) \cdot (3^2 \cdot 3) \cdot 5^2 \cdot 11}= 2^3 \cdot 3 \cdot 5 \sqrt{2 \cdot 3 \cdot 11}= 120 \sqrt{66}
	\]
\end{enumerate}



\newpage



% Problem 9
\problem{10} Showing all your work, simplify the following as much as possible:
        \begin{enumerate}[(a)]
        \item $\sqrt[3]{40}$
        \item $\sqrt[4]{80}$
        \item $\sqrt[3]{2^8 \cdot 3^2 \cdot 5 \cdot 7^6}$
        \item $\sqrt[5]{2^4 \cdot 5^{10} \cdot 7^5}$
        \end{enumerate} \pspace

\sol
\begin{enumerate}[(a)]
\item 
	\[
	\sqrt[3]{40}= \sqrt[3]{2^3 \cdot 5}= 2 \sqrt[3]{5}
	\] \pspace

\item 
	\[
	\sqrt[4]{80}= \sqrt[4]{2^4 \cdot 5}= 2 \sqrt[4]{5}
	\] \pspace

\item \[
	\sqrt[3]{2^8 \cdot 3^2 \cdot 5 \cdot 7^6}= \sqrt[3]{(2^6 \cdot 2^2) \cdot 3^2 \cdot 5 \cdot 7^6}= 2^2 \cdot 7^2 \sqrt[3]{2^2 \cdot 3^2 \cdot 5}= 196 \sqrt[3]{180}
	\] \pspace

\item \[
	\sqrt[5]{2^4 \cdot 5^{10} \cdot 7^5}= 5^2 \cdot 7^1 \sqrt[5]{2^4}= 175 \sqrt[5]{16}
	\]
\end{enumerate}



\newpage



% Problem 10
\problem{10} Rationalize the following fractions:
        \begin{enumerate}[(a)]
        \item $\dfrac{1}{\sqrt{11}}$
        \item $\dfrac{4}{\sqrt{13}}$
        \item $\dfrac{5}{3 + \sqrt{7}}$
        \item $\dfrac{1}{\sqrt[5]{3}}$
        \end{enumerate} \pspace

\sol
\begin{enumerate}[(a)]
\item 
	\[
	\dfrac{1}{\sqrt{11}}= \dfrac{1}{\sqrt{11}} \cdot \dfrac{\sqrt{11}}{\sqrt{11}}= \dfrac{\sqrt{11}}{11}
	\] \pspace

\item 
	\[
	\dfrac{4}{\sqrt{13}}= \dfrac{4}{\sqrt{13}} \cdot \dfrac{\sqrt{13}}{\sqrt{13}}= \dfrac{4 \sqrt{13}}{13}
	\] \pspace

\item 
	\[
	\dfrac{5}{3 + \sqrt{7}}= \dfrac{5}{3 + \sqrt{7}} \cdot \dfrac{3 - \sqrt{7}}{3 - \sqrt{7}}= \dfrac{15 - 5\sqrt{7}}{9 - 3\sqrt{7} + 3\sqrt{7} - 7}= \dfrac{15 - 5\sqrt{7}}{2}
	\] \pspace

\item 
	\[
	\dfrac{1}{\sqrt[5]{3}}= \dfrac{1}{3^{1/5}}= \dfrac{1}{3^{1/5}} \cdot \dfrac{3^{4/5}}{3^{4/5}}= \dfrac{3^{4/5}}{3^1}= \dfrac{\sqrt[5]{3^4}}{3}= \dfrac{\sqrt[5]{81}}{3}
	\]
\end{enumerate}


\end{document}